Test/SelfHosting/Main.cs
@@ -1,4 +1,5 @@
 using Antlr4.Runtime;
+using CSharpAST;
 
 namespace SelfHosting.CSharp;
 
