Test/SelfHosting/CSharpCompat.dfy
@@ -1,15 +1,44 @@
 module {:extern "System.Collections.Generic"} CSharpGenerics {
-  class {:extern "List"} List<T> {}
+  class {:extern} List<T> {}
+  class {:extern} ISet<T> {}
+  class {:extern} HashSet<T> {}
+  class {:extern} Dictionary<TKey, TValue> {}
+  class {:extern} Tuple2<T1, T2> {}
+  class {:extern} Tuple3<T1, T2, T3> {}
+}
+
+module {:extern "System"} CSharpSystem {
+  trait {:compile false} {:termination false} {:extern} IComparable {}
+  class {:extern} Func<TArg, TRet>{}
+  class {:extern} String {}
+}
+
+module {:extern "Microsoft.Dafny"} Dafny {
+  class {:extern} FreshIdGenerator {}
+  class {:extern} Graph<T> {}
+  class {:extern} Translator {}
+  class {:extern} VisibilityScope {}
+}
+
+module {:extern "Microsoft.Dafny.Resolver"} DafnyResolver {
+  class {:extern} TypeConstraint {}
+}
+
+module {:extern "Microsoft.Boogie"} Boogie {
+  trait {:compile false} {:extern} {:termination false} IToken {}
+  class {:extern} ErrorReporter {}
+  class {:extern} Expr {}
+  class {:extern} Function {}
 }
 
 module {:extern "SelfHosting.CSharpUtils"} CSharpUtils {
   import opened CSharpGenerics
 
   class ListUtils {
-    static function method {:extern "FoldR"} FoldR<A, B>(f: (A, B) -> B, b0: B, l: List<A>) : B
+    static function method {:extern} FoldR<A, B>(f: (A, B) -> B, b0: B, l: List<A>) : B
 
-    static method {:extern "Mk"} Mk<T>() returns (l: List<T>)
-    static method {:extern "Append"} Append<T>(l: List<T>, t: T)
+    static method {:extern} Mk<T>() returns (l: List<T>)
+    static method {:extern} Append<T>(l: List<T>, t: T)
 
     static method AppendSeq<T>(l: List<T>, s:seq<T>) {
       var i := 0;
